theories/simplang/heap_bij.v
@@ -15,13 +15,14 @@ Section fix_heap.
 
   Global Program Instance heap_bij_inv : sheapInv Σ := {|
     sheap_inv _ _ _:= ∃ L, heap_bij_interp L (λ _ _ q, q = Some 1%Qp);
+    sheap_ext_rel _ := val_rel;
   |}%I.
   Next Obligation. done. Qed.
   Global Instance : sheapInvSupportsAll.
   Proof. done. Qed.
 
-  Local Notation "et '⪯' es {{ Φ }}" := (et ⪯{π, const val_rel} es {{Φ}})%I (at level 40, Φ at level 200) : bi_scope.
-  Local Notation "et '⪯' es [{ Φ }]" := (et ⪯{π, const val_rel} es [{Φ}])%I (at level 40, Φ at level 200) : bi_scope.
+  Local Notation "et '⪯' es {{ Φ }}" := (et ⪯{π} es {{Φ}})%I (at level 40, Φ at level 200) : bi_scope.
+  Local Notation "et '⪯' es [{ Φ }]" := (et ⪯{π} es [{Φ}])%I (at level 40, Φ at level 200) : bi_scope.
 
   Lemma sim_bij_load_sc l_t l_s Φ :
     l_t ↔h l_s -∗
@@ -249,7 +250,7 @@ Section sim.
 
   Import bi.
 
-  Local Notation "et '⪯' es {{ Φ }}" := (et ⪯{π, const val_rel} es {{Φ}})%I (at level 40, Φ at level 200) : bi_scope.
+  Local Notation "et '⪯' es {{ Φ }}" := (et ⪯{π} es {{Φ}})%I (at level 40, Φ at level 200) : bi_scope.
 
   Implicit Types
     (K_t K_s : ectx)
@@ -268,10 +269,10 @@ Section sim.
     (∀ v_t v_s,
       match envs_app true (Esnoc Enil j (val_rel v_t v_s)) Δ with
       | Some Δ' =>
-          envs_entails Δ' (sim_expr (const val_rel) Φ π (fill K_t (Val v_t)) (fill K_s (Val v_s)))
+          envs_entails Δ' (sim_expr Φ π (fill K_t (Val v_t)) (fill K_s (Val v_s)))
       | None => False
       end) →
-    envs_entails Δ (sim_expr (const val_rel) Φ π (fill K_t (Load o (LitV l_t))) (fill K_s (Load o (LitV l_s))))%I.
+    envs_entails Δ (sim_expr Φ π (fill K_t (Load o (LitV l_t))) (fill K_s (Load o (LitV l_s))))%I.
   Proof.
     rewrite envs_entails_eq=> ? Hi.
     rewrite -sim_expr_bind. eapply wand_apply; first exact: sim_bij_load.
@@ -287,8 +288,8 @@ Section sim.
   Lemma tac_bij_store Δ i K_t K_s b l_t l_s v_t' v_s' o Φ :
     envs_lookup i Δ = Some (b, l_t ↔h l_s)%I →
     envs_entails Δ (val_rel v_t' v_s') →
-    envs_entails Δ (sim_expr (const val_rel) Φ π (fill K_t (Val $ LitV LitUnit)) (fill K_s (Val $ LitV LitUnit))) →
-    envs_entails Δ (sim_expr (const val_rel) Φ π (fill K_t (Store o (LitV l_t) (Val v_t'))) (fill K_s (Store o (LitV l_s) (Val v_s')))).
+    envs_entails Δ (sim_expr Φ π (fill K_t (Val $ LitV LitUnit)) (fill K_s (Val $ LitV LitUnit))) →
+    envs_entails Δ (sim_expr Φ π (fill K_t (Store o (LitV l_t) (Val v_t'))) (fill K_s (Store o (LitV l_s) (Val v_s')))).
   Proof.
     rewrite envs_entails_eq => HΔ.
     rewrite (persistent_persistently_2 (val_rel _ _)).
@@ -307,8 +308,8 @@ Section sim.
     *)
   Lemma tac_bij_freeN Δ i K_t K_s b l_t l_s n Φ :
     envs_lookup i Δ = Some (b, l_t ↔h l_s)%I →
-    envs_entails (envs_delete true i b Δ) (sim_expr (const val_rel) Φ π (fill K_t (Val $ LitV LitUnit)) (fill K_s (Val $ LitV LitUnit))) →
-    envs_entails Δ (sim_expr (const val_rel) Φ π (fill K_t (FreeN (Val $ LitV $ LitInt n) (LitV l_t))) (fill K_s (FreeN (Val $ LitV $ LitInt n) (LitV l_s)))).
+    envs_entails (envs_delete true i b Δ) (sim_expr Φ π (fill K_t (Val $ LitV LitUnit)) (fill K_s (Val $ LitV LitUnit))) →
+    envs_entails Δ (sim_expr Φ π (fill K_t (FreeN (Val $ LitV $ LitInt n) (LitV l_t))) (fill K_s (FreeN (Val $ LitV $ LitInt n) (LitV l_s)))).
   Proof.
     rewrite envs_entails_eq => Hl HΔ.
     rewrite -sim_expr_bind. rewrite (envs_lookup_sound _ _ _ _ Hl).
@@ -329,7 +330,7 @@ Tactic Notation "sim_load" ident(v_t) ident(v_s) "as" constr(H) :=
     pm_reduce; sim_finish in
   sim_pures_int;
   lazymatch goal with
-  | |- envs_entails _ (sim_expr ?vrel ?Φ ?π ?e_t ?e_s) =>
+  | |- envs_entails _ (sim_expr ?Φ ?π ?e_t ?e_s) =>
     first
       [reshape_expr e_t ltac:(fun K_t e_t' =>
         reshape_expr e_s ltac:(fun K_s e_s' =>
@@ -350,7 +351,7 @@ Tactic Notation "sim_store" :=
     iAssumptionCore || fail "sim_store: cannot find" l_t "↔h" l_s end in
   sim_pures_int;
   lazymatch goal with
-  | |- envs_entails _ (sim_expr ?vrel ?Φ ?π ?e_t ?e_s) =>
+  | |- envs_entails _ (sim_expr ?Φ ?π ?e_t ?e_s) =>
     first
       [reshape_expr e_t ltac:(fun K_t e_t' =>
         reshape_expr e_s ltac:(fun K_s e_s' =>
@@ -369,7 +370,7 @@ Tactic Notation "sim_free" :=
     iAssumptionCore || fail "sim_free: cannot find" l_t "↔h" l_s end in
   sim_pures_int;
   lazymatch goal with
-  | |- envs_entails _ (sim_expr ?vrel ?Φ ?π ?e_t ?e_s) =>
+  | |- envs_entails _ (sim_expr ?Φ ?π ?e_t ?e_s) =>
     first
       [reshape_expr e_t ltac:(fun K_t e_t' =>
         reshape_expr e_s ltac:(fun K_s e_s' =>
